Code works nicely

code/Spectre.hs
@@ -1,0 +1,570 @@
+{-# LANGUAGE EmptyDataDecls, RankNTypes, ScopedTypeVariables #-}
+
+module Spectre(Int, Pre_digraph_ext, vote_Spectre_Int) where {
+
+import Prelude ((==), (/=), (<), (<=), (>=), (>), (+), (-), (*), (/), (**),
+  (>>=), (>>), (=<<), (&&), (||), (^), (^^), (.), ($), ($!), (++), (!!), Eq,
+  error, id, return, not, fst, snd, map, filter, concat, concatMap, reverse,
+  zip, null, takeWhile, dropWhile, all, any, Integer, negate, abs, divMod,
+  String, Bool(True, False), Maybe(Nothing, Just));
+import qualified Prelude;
+
+data Num = One | Bit0 Num | Bit1 Num;
+
+data Int = Zero_int | Pos Num | Neg Num;
+
+one_int :: Int;
+one_int = Pos One;
+
+class One a where {
+  one :: a;
+};
+
+instance One Int where {
+  one = one_int;
+};
+
+class Zero a where {
+  zero :: a;
+};
+
+instance Zero Int where {
+  zero = Zero_int;
+};
+
+class (One a, Zero a) => Zero_neq_one a where {
+};
+
+instance Zero_neq_one Int where {
+};
+
+class Ord a where {
+  less_eq :: a -> a -> Bool;
+  less :: a -> a -> Bool;
+};
+
+instance Ord Integer where {
+  less_eq = (\ a b -> a <= b);
+  less = (\ a b -> a < b);
+};
+
+class (Ord a) => Preorder a where {
+};
+
+class (Preorder a) => Order a where {
+};
+
+instance Preorder Integer where {
+};
+
+instance Order Integer where {
+};
+
+class (Order a) => Linorder a where {
+};
+
+instance Linorder Integer where {
+};
+
+data Nat = Zero_nat | Suc Nat;
+
+data Set a = Set [a] | Coset [a];
+
+data Pre_digraph_ext a b c =
+  Pre_digraph_ext (Set a) (Set b) (b -> a) (b -> a) c;
+
+dup :: Int -> Int;
+dup (Neg n) = Neg (Bit0 n);
+dup (Pos n) = Pos (Bit0 n);
+dup Zero_int = Zero_int;
+
+uminus_int :: Int -> Int;
+uminus_int (Neg m) = Pos m;
+uminus_int (Pos m) = Neg m;
+uminus_int Zero_int = Zero_int;
+
+plus_num :: Num -> Num -> Num;
+plus_num (Bit1 m) (Bit1 n) = Bit0 (plus_num (plus_num m n) One);
+plus_num (Bit1 m) (Bit0 n) = Bit1 (plus_num m n);
+plus_num (Bit1 m) One = Bit0 (plus_num m One);
+plus_num (Bit0 m) (Bit1 n) = Bit1 (plus_num m n);
+plus_num (Bit0 m) (Bit0 n) = Bit0 (plus_num m n);
+plus_num (Bit0 m) One = Bit1 m;
+plus_num One (Bit1 n) = Bit0 (plus_num n One);
+plus_num One (Bit0 n) = Bit1 n;
+plus_num One One = Bit0 One;
+
+bitM :: Num -> Num;
+bitM One = One;
+bitM (Bit0 n) = Bit1 (bitM n);
+bitM (Bit1 n) = Bit1 (Bit0 n);
+
+sub :: Num -> Num -> Int;
+sub (Bit0 m) (Bit1 n) = minus_int (dup (sub m n)) one_int;
+sub (Bit1 m) (Bit0 n) = plus_int (dup (sub m n)) one_int;
+sub (Bit1 m) (Bit1 n) = dup (sub m n);
+sub (Bit0 m) (Bit0 n) = dup (sub m n);
+sub One (Bit1 n) = Neg (Bit0 n);
+sub One (Bit0 n) = Neg (bitM n);
+sub (Bit1 m) One = Pos (Bit0 m);
+sub (Bit0 m) One = Pos (bitM m);
+sub One One = Zero_int;
+
+plus_int :: Int -> Int -> Int;
+plus_int (Neg m) (Neg n) = Neg (plus_num m n);
+plus_int (Neg m) (Pos n) = sub n m;
+plus_int (Pos m) (Neg n) = sub m n;
+plus_int (Pos m) (Pos n) = Pos (plus_num m n);
+plus_int Zero_int l = l;
+plus_int k Zero_int = k;
+
+minus_int :: Int -> Int -> Int;
+minus_int (Neg m) (Neg n) = sub n m;
+minus_int (Neg m) (Pos n) = Neg (plus_num m n);
+minus_int (Pos m) (Neg n) = Pos (plus_num m n);
+minus_int (Pos m) (Pos n) = sub m n;
+minus_int Zero_int l = uminus_int l;
+minus_int k Zero_int = k;
+
+bex :: forall a. Set a -> (a -> Bool) -> Bool;
+bex (Set xs) p = any p xs;
+
+minus_nat :: Nat -> Nat -> Nat;
+minus_nat (Suc m) (Suc n) = minus_nat m n;
+minus_nat Zero_nat n = Zero_nat;
+minus_nat m Zero_nat = m;
+
+membera :: forall a. (Eq a) => [a] -> a -> Bool;
+membera [] y = False;
+membera (x : xs) y = x == y || membera xs y;
+
+member :: forall a. (Eq a) => a -> Set a -> Bool;
+member x (Coset xs) = not (membera xs x);
+member x (Set xs) = membera xs x;
+
+removeAll :: forall a. (Eq a) => a -> [a] -> [a];
+removeAll x [] = [];
+removeAll x (y : xs) = (if x == y then removeAll x xs else y : removeAll x xs);
+
+inserta :: forall a. (Eq a) => a -> [a] -> [a];
+inserta x xs = (if membera xs x then xs else x : xs);
+
+insert :: forall a. (Eq a) => a -> Set a -> Set a;
+insert x (Coset xs) = Coset (removeAll x xs);
+insert x (Set xs) = Set (inserta x xs);
+
+fold :: forall a b. (a -> b -> b) -> [a] -> b -> b;
+fold f (x : xs) s = fold f xs (f x s);
+fold f [] s = s;
+
+sup_set :: forall a. (Eq a) => Set a -> Set a -> Set a;
+sup_set (Coset xs) a = Coset (filter (\ x -> not (member x a)) xs);
+sup_set (Set xs) a = fold insert xs a;
+
+relcomp :: forall a b c. (Eq b) => Set (a, b) -> Set (b, c) -> Set (a, c);
+relcomp (Set xys) (Set yzs) =
+  Set (concatMap
+        (\ xy ->
+          concatMap
+            (\ yz -> (if snd xy == fst yz then [(fst xy, snd yz)] else [])) yzs)
+        xys);
+
+ntrancl :: forall a. (Eq a) => Nat -> Set (a, a) -> Set (a, a);
+ntrancl (Suc n) r = let {
+                      ra = ntrancl n r;
+                    } in sup_set ra (relcomp ra r);
+ntrancl Zero_nat r = r;
+
+one_nat :: Nat;
+one_nat = Suc Zero_nat;
+
+gen_length :: forall a. Nat -> [a] -> Nat;
+gen_length n (x : xs) = gen_length (Suc n) xs;
+gen_length n [] = n;
+
+size_list :: forall a. [a] -> Nat;
+size_list = gen_length Zero_nat;
+
+remdups :: forall a. (Eq a) => [a] -> [a];
+remdups [] = [];
+remdups (x : xs) = (if membera xs x then remdups xs else x : remdups xs);
+
+card :: forall a. (Eq a) => Set a -> Nat;
+card (Set xs) = size_list (remdups xs);
+
+trancl :: forall a. (Eq a) => Set (a, a) -> Set (a, a);
+trancl (Set xs) = ntrancl (minus_nat (card (Set xs)) one_nat) (Set xs);
+
+verts :: forall a b c. Pre_digraph_ext a b c -> Set a;
+verts (Pre_digraph_ext verts arcs tail head more) = verts;
+
+arcs :: forall a b c. Pre_digraph_ext a b c -> Set b;
+arcs (Pre_digraph_ext verts arcs tail head more) = arcs;
+
+tail :: forall a b c. Pre_digraph_ext a b c -> b -> a;
+tail (Pre_digraph_ext verts arcs tail head more) = tail;
+
+head :: forall a b c. Pre_digraph_ext a b c -> b -> a;
+head (Pre_digraph_ext verts arcs tail head more) = head;
+
+arc_to_ends :: forall a b. Pre_digraph_ext a b () -> b -> (a, a);
+arc_to_ends g e = (tail g e, head g e);
+
+image :: forall a b. (a -> b) -> Set a -> Set b;
+image f (Set xs) = Set (map f xs);
+
+arcs_ends :: forall a b. Pre_digraph_ext a b () -> Set (a, a);
+arcs_ends g = image (arc_to_ends g) (arcs g);
+
+ball :: forall a. Set a -> (a -> Bool) -> Bool;
+ball (Set xs) p = all p xs;
+
+wf_digraph :: forall a b. (Eq a) => Pre_digraph_ext a b () -> Bool;
+wf_digraph g =
+  ball (arcs g) (\ e -> member (tail g e) (verts g)) &&
+    ball (arcs g) (\ e -> member (head g e) (verts g));
+
+loopfree_digraph :: forall a b. (Eq a) => Pre_digraph_ext a b () -> Bool;
+loopfree_digraph g =
+  wf_digraph g && ball (arcs g) (\ e -> not (tail g e == head g e));
+
+nomulti_digraph :: forall a b. (Eq a, Eq b) => Pre_digraph_ext a b () -> Bool;
+nomulti_digraph g =
+  wf_digraph g &&
+    ball (arcs g)
+      (\ e1 ->
+        ball (arcs g)
+          (\ e2 ->
+            (if arc_to_ends g e1 == arc_to_ends g e2 then e1 == e2 else True)));
+
+less_nat :: Nat -> Nat -> Bool;
+less_nat m (Suc n) = less_eq_nat m n;
+less_nat n Zero_nat = False;
+
+less_eq_nat :: Nat -> Nat -> Bool;
+less_eq_nat (Suc m) n = less_nat m n;
+less_eq_nat Zero_nat n = True;
+
+is_empty :: forall a. Set a -> Bool;
+is_empty (Set xs) = null xs;
+
+fin_digraph :: forall a b. (Eq a, Eq b) => Pre_digraph_ext a b () -> Bool;
+fin_digraph g =
+  wf_digraph g &&
+    (less_nat Zero_nat (card (verts g)) || is_empty (verts g)) &&
+      (less_nat Zero_nat (card (arcs g)) || is_empty (arcs g));
+
+digraph :: forall a b. (Eq a, Eq b) => Pre_digraph_ext a b () -> Bool;
+digraph g = fin_digraph g && loopfree_digraph g && nomulti_digraph g;
+
+dag :: forall a b. (Eq a, Eq b) => Pre_digraph_ext a b () -> Bool;
+dag g =
+  digraph g &&
+    ball (verts g) (\ v -> not (member (v, v) (trancl (arcs_ends g))));
+
+nth :: forall a. [a] -> Nat -> a;
+nth (x : xs) (Suc n) = nth xs n;
+nth (x : xs) Zero_nat = x;
+
+filtera :: forall a. (a -> Bool) -> Set a -> Set a;
+filtera p (Set xs) = Set (filter p xs);
+
+remove :: forall a. (Eq a) => a -> Set a -> Set a;
+remove x (Coset xs) = Coset (inserta x xs);
+remove x (Set xs) = Set (removeAll x xs);
+
+arcAlt ::
+  forall a b. (Eq a, Eq b) => Pre_digraph_ext a b () -> b -> (a, a) -> Bool;
+arcAlt g e uv = member e (arcs g) && tail g e == fst uv && head g e == snd uv;
+
+plus_nat :: Nat -> Nat -> Nat;
+plus_nat (Suc m) n = plus_nat m (Suc n);
+plus_nat Zero_nat n = n;
+
+nat_of_num :: Num -> Nat;
+nat_of_num (Bit1 n) = let {
+                        m = nat_of_num n;
+                      } in Suc (plus_nat m m);
+nat_of_num (Bit0 n) = let {
+                        m = nat_of_num n;
+                      } in plus_nat m m;
+nat_of_num One = one_nat;
+
+past_nodes :: forall a b. (Eq a) => Pre_digraph_ext a b () -> a -> Set a;
+past_nodes g a =
+  filtera (\ b -> member (a, b) (trancl (arcs_ends g))) (verts g);
+
+induce_subgraph ::
+  forall a b.
+    (Eq a) => Pre_digraph_ext a b () -> Set a -> Pre_digraph_ext a b ();
+induce_subgraph g vs =
+  Pre_digraph_ext vs
+    (filtera (\ e -> member (tail g e) vs && member (head g e) vs) (arcs g))
+    (tail g) (head g) ();
+
+reduce_past ::
+  forall a b. (Eq a) => Pre_digraph_ext a b () -> a -> Pre_digraph_ext a b ();
+reduce_past g a = induce_subgraph g (past_nodes g a);
+
+future_nodes :: forall a b. (Eq a) => Pre_digraph_ext a b () -> a -> Set a;
+future_nodes g a =
+  filtera (\ b -> member (b, a) (trancl (arcs_ends g))) (verts g);
+
+del_arc ::
+  forall a b. (Eq b) => Pre_digraph_ext a b () -> b -> Pre_digraph_ext a b ();
+del_arc g a =
+  Pre_digraph_ext (verts g) (remove a (arcs g)) (tail g) (head g) ();
+
+blockDAG :: forall a b. (Eq a, Eq b) => Pre_digraph_ext a b () -> Bool;
+blockDAG g =
+  dag g &&
+    bex (verts g)
+      (\ p ->
+        ball (verts g)
+          (\ r -> member (r, p) (trancl (arcs_ends g)) || r == p)) &&
+      ball (arcs g)
+        (\ e ->
+          ball (verts g)
+            (\ u ->
+              ball (verts g)
+                (\ v ->
+                  (if member (u, v) (trancl (arcs_ends (del_arc g e)))
+                    then not (arcAlt g e (u, v)) else True))));
+
+of_bool :: forall a. (Zero_neq_one a) => Bool -> a;
+of_bool True = one;
+of_bool False = zero;
+
+equal_num :: Num -> Num -> Bool;
+equal_num (Bit0 x2) (Bit1 x3) = False;
+equal_num (Bit1 x3) (Bit0 x2) = False;
+equal_num One (Bit1 x3) = False;
+equal_num (Bit1 x3) One = False;
+equal_num One (Bit0 x2) = False;
+equal_num (Bit0 x2) One = False;
+equal_num (Bit1 x3) (Bit1 y3) = equal_num x3 y3;
+equal_num (Bit0 x2) (Bit0 y2) = equal_num x2 y2;
+equal_num One One = True;
+
+equal_int :: Int -> Int -> Bool;
+equal_int (Neg k) (Neg l) = equal_num k l;
+equal_int (Neg k) (Pos l) = False;
+equal_int (Neg k) Zero_int = False;
+equal_int (Pos k) (Neg l) = False;
+equal_int (Pos k) (Pos l) = equal_num k l;
+equal_int (Pos k) Zero_int = False;
+equal_int Zero_int (Neg l) = False;
+equal_int Zero_int (Pos l) = False;
+equal_int Zero_int Zero_int = True;
+
+adjust_div :: (Int, Int) -> Int;
+adjust_div (q, r) = plus_int q (of_bool (not (equal_int r Zero_int)));
+
+adjust_mod :: Int -> Int -> Int;
+adjust_mod l r = (if equal_int r Zero_int then Zero_int else minus_int l r);
+
+equal_nat :: Nat -> Nat -> Bool;
+equal_nat Zero_nat (Suc x2) = False;
+equal_nat (Suc x2) Zero_nat = False;
+equal_nat (Suc x2) (Suc y2) = equal_nat x2 y2;
+equal_nat Zero_nat Zero_nat = True;
+
+divmod_nat :: Nat -> Nat -> (Nat, Nat);
+divmod_nat m n =
+  (if equal_nat n Zero_nat || less_nat m n then (Zero_nat, m)
+    else let {
+           a = divmod_nat (minus_nat m n) n;
+         } in (case a of {
+                (q, aa) -> (Suc q, aa);
+              }));
+
+divide_nat :: Nat -> Nat -> Nat;
+divide_nat m n = fst (divmod_nat m n);
+
+part :: forall a b. (Linorder b) => (a -> b) -> b -> [a] -> ([a], ([a], [a]));
+part f pivot (x : xs) =
+  (case part f pivot xs of {
+    (lts, (eqs, gts)) ->
+      let {
+        xa = f x;
+      } in (if less xa pivot then (x : lts, (eqs, gts))
+             else (if less pivot xa then (lts, (eqs, x : gts))
+                    else (lts, (x : eqs, gts))));
+  });
+part f pivot [] = ([], ([], []));
+
+sort_key :: forall a b. (Linorder b) => (a -> b) -> [a] -> [a];
+sort_key f xs =
+  (case xs of {
+    [] -> [];
+    [_] -> xs;
+    [x, y] -> (if less_eq (f x) (f y) then xs else [y, x]);
+    _ : _ : _ : _ ->
+      (case part f
+              (f (nth xs (divide_nat (size_list xs) (nat_of_num (Bit0 One)))))
+              xs
+        of {
+        (lts, (eqs, gts)) -> sort_key f lts ++ eqs ++ sort_key f gts;
+      });
+  });
+
+sorted_list_of_set :: forall a. (Eq a, Linorder a) => Set a -> [a];
+sorted_list_of_set (Set xs) = sort_key (\ x -> x) (remdups xs);
+
+less_num :: Num -> Num -> Bool;
+less_num (Bit1 m) (Bit0 n) = less_num m n;
+less_num (Bit1 m) (Bit1 n) = less_num m n;
+less_num (Bit0 m) (Bit1 n) = less_eq_num m n;
+less_num (Bit0 m) (Bit0 n) = less_num m n;
+less_num One (Bit1 n) = True;
+less_num One (Bit0 n) = True;
+less_num m One = False;
+
+less_eq_num :: Num -> Num -> Bool;
+less_eq_num (Bit1 m) (Bit0 n) = less_num m n;
+less_eq_num (Bit1 m) (Bit1 n) = less_eq_num m n;
+less_eq_num (Bit0 m) (Bit1 n) = less_eq_num m n;
+less_eq_num (Bit0 m) (Bit0 n) = less_eq_num m n;
+less_eq_num (Bit1 m) One = False;
+less_eq_num (Bit0 m) One = False;
+less_eq_num One n = True;
+
+less_int :: Int -> Int -> Bool;
+less_int (Neg k) (Neg l) = less_num l k;
+less_int (Neg k) (Pos l) = True;
+less_int (Neg k) Zero_int = True;
+less_int (Pos k) (Neg l) = False;
+less_int (Pos k) (Pos l) = less_num k l;
+less_int (Pos k) Zero_int = False;
+less_int Zero_int (Neg l) = False;
+less_int Zero_int (Pos l) = True;
+less_int Zero_int Zero_int = False;
+
+tie_break_int :: forall a. (Linorder a) => a -> a -> Int -> Int;
+tie_break_int a b i =
+  (if equal_int i Zero_int
+    then (if less b a then uminus_int one_int else one_int)
+    else (if less_int Zero_int i then one_int else uminus_int one_int));
+
+sumlist_break_acc :: forall a. (Linorder a) => a -> a -> Int -> [Int] -> Int;
+sumlist_break_acc a b s [] = tie_break_int a b s;
+sumlist_break_acc a b s (x : xs) = sumlist_break_acc a b (plus_int s x) xs;
+
+sumlist_break :: forall a. (Linorder a) => a -> a -> [Int] -> Int;
+sumlist_break a b [] = Zero_int;
+sumlist_break a b (x : xs) = sumlist_break_acc a b Zero_int (x : xs);
+
+vote_Spectre ::
+  forall a b.
+    (Eq a, Linorder a, Eq b) => Pre_digraph_ext a b () -> a -> a -> a -> Int;
+vote_Spectre v a b c =
+  (if not (blockDAG v) ||
+        (not (member a (verts v)) ||
+          (not (member b (verts v)) || not (member c (verts v))))
+    then Zero_int
+    else (if b == c then one_int
+           else (if (member (a, b) (trancl (arcs_ends v)) || a == b) &&
+                      not (member (a, c) (trancl (arcs_ends v)))
+                  then one_int
+                  else (if (member (a, c) (trancl (arcs_ends v)) || a == c) &&
+                             not (member (a, b) (trancl (arcs_ends v)))
+                         then uminus_int one_int
+                         else (if member (a, b) (trancl (arcs_ends v)) &&
+                                    member (a, c) (trancl (arcs_ends v))
+                                then sumlist_break b c
+                                       (map
+ (\ i -> vote_Spectre (reduce_past v a) i b c)
+ (sorted_list_of_set (past_nodes v a)))
+                                else sumlist_break b c
+                                       (map (\ i -> vote_Spectre v i b c)
+ (sorted_list_of_set (future_nodes v a))))))));
+
+times_num :: Num -> Num -> Num;
+times_num (Bit1 m) (Bit1 n) =
+  Bit1 (plus_num (plus_num m n) (Bit0 (times_num m n)));
+times_num (Bit1 m) (Bit0 n) = Bit0 (times_num (Bit1 m) n);
+times_num (Bit0 m) (Bit1 n) = Bit0 (times_num m (Bit1 n));
+times_num (Bit0 m) (Bit0 n) = Bit0 (Bit0 (times_num m n));
+times_num One n = n;
+times_num m One = m;
+
+times_int :: Int -> Int -> Int;
+times_int (Neg m) (Neg n) = Pos (times_num m n);
+times_int (Neg m) (Pos n) = Neg (times_num m n);
+times_int (Pos m) (Neg n) = Neg (times_num m n);
+times_int (Pos m) (Pos n) = Pos (times_num m n);
+times_int Zero_int l = Zero_int;
+times_int k Zero_int = Zero_int;
+
+less_eq_int :: Int -> Int -> Bool;
+less_eq_int (Neg k) (Neg l) = less_eq_num l k;
+less_eq_int (Neg k) (Pos l) = True;
+less_eq_int (Neg k) Zero_int = True;
+less_eq_int (Pos k) (Neg l) = False;
+less_eq_int (Pos k) (Pos l) = less_eq_num k l;
+less_eq_int (Pos k) Zero_int = False;
+less_eq_int Zero_int (Neg l) = False;
+less_eq_int Zero_int (Pos l) = True;
+less_eq_int Zero_int Zero_int = True;
+
+divmod_step_int :: Num -> (Int, Int) -> (Int, Int);
+divmod_step_int l (q, r) =
+  (if less_eq_int (Pos l) r
+    then (plus_int (times_int (Pos (Bit0 One)) q) one_int, minus_int r (Pos l))
+    else (times_int (Pos (Bit0 One)) q, r));
+
+divmod_int :: Num -> Num -> (Int, Int);
+divmod_int (Bit1 m) (Bit1 n) =
+  (if less_num m n then (Zero_int, Pos (Bit1 m))
+    else divmod_step_int (Bit1 n) (divmod_int (Bit1 m) (Bit0 (Bit1 n))));
+divmod_int (Bit0 m) (Bit1 n) =
+  (if less_eq_num m n then (Zero_int, Pos (Bit0 m))
+    else divmod_step_int (Bit1 n) (divmod_int (Bit0 m) (Bit0 (Bit1 n))));
+divmod_int (Bit1 m) (Bit0 n) =
+  (case divmod_int m n of {
+    (q, r) -> (q, plus_int (times_int (Pos (Bit0 One)) r) one_int);
+  });
+divmod_int (Bit0 m) (Bit0 n) = (case divmod_int m n of {
+                                 (q, r) -> (q, times_int (Pos (Bit0 One)) r);
+                               });
+divmod_int One (Bit1 n) = (Zero_int, Pos One);
+divmod_int One (Bit0 n) = (Zero_int, Pos One);
+divmod_int m One = (Pos m, Zero_int);
+
+modulo_int :: Int -> Int -> Int;
+modulo_int (Neg m) (Neg n) = uminus_int (snd (divmod_int m n));
+modulo_int (Pos m) (Neg n) =
+  uminus_int (adjust_mod (Pos n) (snd (divmod_int m n)));
+modulo_int (Neg m) (Pos n) = adjust_mod (Pos n) (snd (divmod_int m n));
+modulo_int (Pos m) (Pos n) = snd (divmod_int m n);
+modulo_int k (Neg One) = Zero_int;
+modulo_int k (Pos One) = Zero_int;
+modulo_int Zero_int k = Zero_int;
+modulo_int k Zero_int = k;
+
+divide_int :: Int -> Int -> Int;
+divide_int (Neg m) (Neg n) = fst (divmod_int m n);
+divide_int (Pos m) (Neg n) = uminus_int (adjust_div (divmod_int m n));
+divide_int (Neg m) (Pos n) = uminus_int (adjust_div (divmod_int m n));
+divide_int (Pos m) (Pos n) = fst (divmod_int m n);
+divide_int k (Neg One) = uminus_int k;
+divide_int k (Pos One) = k;
+divide_int Zero_int k = Zero_int;
+divide_int k Zero_int = Zero_int;
+
+integer_of_int :: Int -> Integer;
+integer_of_int k =
+  (if less_int k Zero_int then negate (integer_of_int (uminus_int k))
+    else (if equal_int k Zero_int then (0 :: Integer)
+           else let {
+                  l = (2 :: Integer) *
+                        integer_of_int (divide_int k (Pos (Bit0 One)));
+                  j = modulo_int k (Pos (Bit0 One));
+                } in (if equal_int j Zero_int then l else l + (1 :: Integer))));
+
+vote_Spectre_Int ::
+  Pre_digraph_ext Integer (Integer, Integer) () ->
+    Integer -> Integer -> Integer -> Integer;
+vote_Spectre_Int v a b c = integer_of_int (vote_Spectre v a b c);
+
+}
