code/Test.hs
@@ -1,0 +1,19 @@
+module Test where
+import Spectre
+
+
+
+verts = Spectre.Set [1,2,3]
+edges = Spectre.Set [21,31]
+
+hd 21 = 1
+hd 31 = 1
+hd x = x
+
+tl 21 = 2
+tl 31 = 3
+tl x = x
+
+
+
+
