Codegen.thy
@@ -4,7 +4,7 @@
 
 
 theory Codegen
-  imports blockDAG Spectre
+  imports blockDAG Spectre 
 begin
 
 section \<open>Code Generation\<close>
@@ -12,49 +12,61 @@ section \<open>Code Generation\<close>
 fun arcAlt::  "('a,'b) pre_digraph \<Rightarrow> 'b \<Rightarrow> 'a \<times> 'a \<Rightarrow> bool"
   where "arcAlt G e uv = (e \<in> arcs G \<and> tail G e = fst uv \<and> head G e = snd uv)"
 
-lemma (in DAG) arcAlt_eq:
+fun iterate:: "('a \<Rightarrow> bool) \<Rightarrow> 'a set \<Rightarrow> bool"
+  where  "iterate S P = Finite_Set.fold (\<lambda> r A. S r \<and> A) False P "
+
+lemma (in DAG) arcAlt_eq:                     
   shows "arcAlt G e uv = wf_digraph.arc G e uv"
   unfolding arc_def arcAlt.simps by simp
   
-lemma [code]: "blockDAG G = ((\<exists>p. (p\<in> verts G \<and> (\<forall>r. r \<in> verts G  \<longrightarrow> r \<rightarrow>\<^sup>*\<^bsub>G\<^esub> p))) \<and>
- (\<forall>e u v. arcAlt G e (u,v) \<longrightarrow> \<not>(u \<rightarrow>\<^sup>*\<^bsub>(pre_digraph.del_arc G  e)\<^esub> v)) \<and> DAG G)"
-  unfolding blockDAG_axioms_def blockDAG_def
-  using DAG.arcAlt_eq by metis
+lemma [code]: "blockDAG G = (DAG G \<and> ((\<exists> p \<in> verts G. ((\<forall>r \<in> verts G. (r \<rightarrow>\<^sup>+\<^bsub>G\<^esub> p \<or> r = p)))) \<and>
+ (\<forall>e \<in> (arcs G). \<forall> u \<in> verts G. \<forall> v \<in> verts G. 
+(u \<rightarrow>\<^sup>+\<^bsub>(pre_digraph.del_arc G  e)\<^esub> v) \<longrightarrow> \<not> arcAlt G e (u,v))))" 
+  using  DAG.arcAlt_eq  wf_digraph_def DAG.axioms(1)
+    digraph.axioms(1) fin_digraph.axioms(1) wf_digraph.arcE blockDAG_axioms_def blockDAG_def 
+  by metis
+     
 
-lemma [code]: "DAG G = (digraph G \<and> (\<forall>v. \<not>(v \<rightarrow>\<^sup>+\<^bsub>G\<^esub> v)))"
-  unfolding DAG_axioms_def DAG_def by auto
+lemma [code]: "DAG G = (digraph G \<and> (\<forall>v \<in> verts G. \<not>(v \<rightarrow>\<^sup>+\<^bsub>G\<^esub> v)))"
+  unfolding DAG_axioms_def DAG_def
+  by (metis digraph.axioms(1) fin_digraph.axioms(1) wf_digraph.reachable1_in_verts(1)) 
 
 lemma [code]: "digraph G = (fin_digraph G \<and> loopfree_digraph G \<and> nomulti_digraph G)"
   unfolding digraph_def by auto
-                
-lemma [code]: "fin_digraph G =  (wf_digraph G \<and> finite (verts G) \<and> finite (arcs G))"
-  unfolding fin_digraph_axioms_def fin_digraph_def by simp
 
 lemma [code]: "wf_digraph G = (
- (\<forall>e.   e \<in> arcs G \<longrightarrow> tail G e \<in> verts G) \<and>
- (\<forall>e. e \<in> arcs G \<longrightarrow> head G e \<in> verts G))"
+ (\<forall>e \<in> arcs G. tail G e \<in> verts G) \<and>
+ (\<forall>e \<in> arcs G. head G e \<in> verts G))"
   using wf_digraph_def by auto
 
 lemma [code]: "nomulti_digraph G = (wf_digraph G \<and> 
-  (\<forall>e1 e2. e1 \<in> arcs G \<and> e2 \<in> arcs G \<and>
+  (\<forall>e1 \<in> arcs G. \<forall> e2 \<in> arcs G .
      arc_to_ends G e1 = arc_to_ends G e2 \<longrightarrow> e1 = e2))"
   unfolding nomulti_digraph_def nomulti_digraph_axioms_def by auto
 
-lemma [code]: "loopfree_digraph G = (wf_digraph G \<and> (\<forall>e.  e \<in> arcs G \<longrightarrow> tail G e \<noteq> head G e))"
+lemma [code]: "loopfree_digraph G = (wf_digraph G \<and> (\<forall>e \<in> arcs G.  tail G e \<noteq> head G e))"
   unfolding loopfree_digraph_def loopfree_digraph_axioms_def by auto
 
 lemma [code]: "pre_digraph.del_arc G a =
  \<lparr> verts = verts G, arcs = arcs G - {a}, tail = tail G, head = head G \<rparr>"
   by (simp add: pre_digraph.del_arc_def)
 
-(**DAG.future_nodes, DAG.reduce_past, DAG.past_nodes
-**)
 
-fun future_nodesAlt:: "('a,'b) pre_digraph \<Rightarrow> 'a \<Rightarrow> 'a set" 
-  where "future_nodesAlt G a = {b. b \<rightarrow>\<^sup>+\<^bsub>G\<^esub> a}"
+fun finiteAlt :: "'a set \<Rightarrow> bool"
+  where "finiteAlt a = (a = {} \<or> (\<exists>A \<in> a. \<exists> b \<subseteq> a. a = insert A b \<and> finite b))"
 
-declare rtrancl_on_def [code]
-declare rtrancl_onp.simps [code]
+lemma [code]: "fin_digraph G = (wf_digraph G \<and> (card (verts G) > 0 \<or> verts G = {})
+   \<and> ((card (arcs G) > 0 \<or> arcs G = {})))" 
+  using card_0_eq card_ge_0_finite fin_digraph_def fin_digraph_axioms_def
+  by (metis card_gt_0_iff finite.emptyI)
 
-export_code vote_Spectre in Haskell module_name Spectre
+
+fun vote_Spectre_Int:: "(integer, integer\<times>integer) pre_digraph \<Rightarrow>
+ integer \<Rightarrow> integer \<Rightarrow> integer \<Rightarrow> integer"
+  where "vote_Spectre_Int V a b c = integer_of_int (vote_Spectre V a b c)"
+
+
+export_code snd fst vote_Spectre_Int in Haskell module_name Spectre file "code/"
+
+
 end
